src/coq/LLVMBaseTypes.v
@@ -1,0 +1,43 @@
+(* -------------------------------------------------------------------------- *
+ *                     Vellvm - the Verified LLVM project                     *
+ *                                                                            *
+ *     Copyright (c) 2017 Steve Zdancewic <stevez@cis.upenn.edu>              *
+ *                                                                            *
+ *   This file is distributed under the terms of the GNU General Public       *
+ *   License as published by the Free Software Foundation, either version     *
+ *   3 of the License, or (at your option) any later version.                 *
+ ---------------------------------------------------------------------------- *)
+
+Require Import ZArith List String Omega.
+Require Import compcert.lib.Integers compcert.lib.Floats.
+
+Set Implicit Arguments.
+Set Contextual Implicit.
+
+Open Scope Z_scope.
+
+(* Set up for i1, i32, and i64 *) 
+Module Wordsize1.
+  Definition wordsize := 1%nat.
+  Remark wordsize_not_zero: wordsize <> 0%nat.
+  Proof. unfold wordsize; congruence. Qed.
+End Wordsize1.
+
+Module Int1 := Make(Wordsize1).
+Module Int32 := Integers.Int.
+Module Int64 := Integers.Int64.
+
+Definition int1 := Int1.int.
+Definition int32 := Int32.int.
+Definition int64 := Int64.int.
+
+Definition inttyp (x:Z) : Type :=
+  match x with
+  | 1 => int1
+  | 32 => int32
+  | 64 => int64
+  | _ => False
+  end.
+
+Definition ll_float  := Floats.float32.
+Definition ll_double := Floats.float.
